Update definitions correspondingly to the changes in specification

theories/Section4/CreateTimeRecord.v
@@ -16,7 +16,6 @@ Definition DeltaDaysValid (deltaDays : option Z) : Prop :=
 
 (*>> 4.5.2 CreateTimeRecord <<*)
 Program Definition CreateTimeRecord (hour minute second millisecond microsecond nanosecond : Z) (deltaDays : option Z) 
-  (days_valid : DeltaDaysValid deltaDays)
   (hour_valid : 0 <= hour <= 23) (minute_valid : 0 <= minute <= 59) (second_valid : 0 <= second <= 59)
   (millisecond_valid : 0 <= millisecond <= 999) (microsecond_valid : 0 <= microsecond <= 999) (nanosecond_valid : 0 <= nanosecond <= 999)
     : TimeRecord := 
@@ -30,7 +29,7 @@ Program Definition CreateTimeRecord (hour minute second millisecond microsecond 
   (*>> 2. Assert: IsValidTime(hour, minute, second, millisecond, microsecond, nanosecond). <<*)
   assert IsValidTime hour minute second millisecond microsecond nanosecond = true in
   (*>> 3. Return Time Record { [[Days]]: deltaDays, [[Hour]]: hour, [[Minute]]: minute, [[Second]]: second, [[Millisecond]]: millisecond, [[Microsecond]]: microsecond, [[Nanosecond]]: nanosecond  }. <<*)
-  mkTimeRecord deltaDays' _ hour hour_valid minute minute_valid second second_valid millisecond millisecond_valid microsecond microsecond_valid nanosecond nanosecond_valid.
+  mkTimeRecord deltaDays' hour hour_valid minute minute_valid second second_valid millisecond millisecond_valid microsecond microsecond_valid nanosecond nanosecond_valid.
 
 Next Obligation.
   unfold IsValidTime.
@@ -40,8 +39,4 @@ Next Obligation.
   destruct_with_eqn ((millisecond <? 0) || (millisecond >? 999)); try lia.
   destruct_with_eqn ((microsecond <? 0) || (microsecond >? 999)); try lia.
   destruct_with_eqn ((nanosecond <? 0) || (nanosecond >? 999)); try lia.
-Qed.
-
-Next Obligation.
-  destruct deltaDays; easy.
 Qed.
