theories/Section11/FormatOffsetTimeZoneIdentifier.v
@@ -9,7 +9,8 @@ Open Scope string_scope.
 Open Scope Z.
 
 (* 11.1.5 FormatOffsetTimeZoneIdentifier *)
-Program Definition FormatOffsetTimeZoneIdentifier (offsetMinutes : Z) (style : option Style) : string :=
+Program Definition FormatOffsetTimeZoneIdentifier 
+  (offsetMinutes : Z) (offsetMinutes_valid : -1439 <= offsetMinutes <= 1439) (style : option Style) : string :=
   (*>> 1. If offsetMinutes ≥ 0, let sign be the code unit 0x002B (PLUS SIGN); otherwise, let sign be the code unit 0x002D (HYPHEN-MINUS). <<*)
   let sign := if offsetMinutes >=? 0 then "+" else "-" in
   (*>> 2. Let absoluteMinutes be abs(offsetMinutes). <<*)
@@ -23,7 +24,23 @@ Program Definition FormatOffsetTimeZoneIdentifier (offsetMinutes : Z) (style : o
   (*>> 6. Return the string-concatenation of sign and timeString. <<*)
   sign ++ timeString.
 
-Next Obligation. Admitted.
+Next Obligation.
+  split.
+  apply Z_div_nonneg_nonneg.
+  apply Z.abs_nonneg.
+  easy.
+  apply Zlt_succ_le.
+  apply Z.div_lt_upper_bound.
+  easy.
+  apply Z.abs_lt.
+  split.
+  apply Z.le_succ_l.
+  easy.
+  apply Z.le_succ_l.
+  apply Z.pred_le_mono.
+  rewrite Z.pred_succ.
+  easy.
+Qed.
 
 Next Obligation.
   split.
