theories/Section4/NoonTimeRecord.v
@@ -5,6 +5,6 @@ Open Scope Z.
 (* 4.5.4 NoonTimeRecord *)
 Program Definition NoonTimeRecord : TimeRecord :=
   (*>> 1. Return Time Record { [[Days]]: 0, [[Hour]]: 12, [[Minute]]: 0, [[Second]]: 0, [[Millisecond]]: 0, [[Microsecond]]: 0, [[Nanosecond]]: 0  }. <<*)
-  mkTimeRecord 0 _ 12 _ 0 _ 0 _ 0 _ 0 _ 0 _.
+  mkTimeRecord 0 12 _ 0 _ 0 _ 0 _ 0 _ 0 _.
 
 Solve Obligations with easy.
